updates

generic/Zeta.Generic.Global.fst
@@ -13,12 +13,12 @@ let evict_sseq (#vspec:_) (gl: verifiable_log vspec)
   : ss:sseq (ms_hashfn_dom vspec.app) { S.length ss = S.length gl }
   = admit()
 
-let appfn_calls
+let app_fcrs
   (#vspec: verifier_spec)
   (gl: verifiable_log vspec): sseq (Zeta.AppSimulate.appfn_call_res vspec.app)
   = admit()
 
-let appfn_calls_within_ep
+let app_fcrs_within_ep
   (#vspec: verifier_spec)
   (ep: epoch)
   (gl: verifiable_log vspec): sseq (Zeta.AppSimulate.appfn_call_res vspec.app)
