high2/Zeta.High.Correctness.fst
@@ -22,18 +22,18 @@ module HG = Zeta.High.Global
 let lemma_verifier_correct
   (#app:_)
   (epmax: epoch)
-  (gl: HG.ms_verifiable_log app epmax{~ (seq_consistent (appfn_calls_within_ep epmax gl)) /\ S.length gl > 0})
+  (gl: HG.ms_verifiable_log app epmax{~ (seq_consistent (app_fcrs_within_ep epmax gl)) /\ S.length gl > 0})
   : hash_collision app
   = (* sequence of sequence of app fn calls and results *)
-    let app_calls_ss = appfn_calls_within_ep epmax gl in
+    let app_calls_ss = app_fcrs_within_ep epmax gl in
 
     (* interleaving of gl ordered by time of each log entry *)
     let itsl = create gl in
 
     (* prefix upto epoch epmax *)
     let itsl_ep = prefix_within_epoch epmax itsl in
-    lemma_appfn_calls_within_epoch epmax itsl;
-    assert(G.appfn_calls (to_glog itsl_ep) = app_calls_ss);
+    lemma_fcrs_within_epoch epmax itsl;
+    assert(G.app_fcrs (to_glog itsl_ep) = app_calls_ss);
 
     lemma_add_evict_set_identical_glog epmax itsl;
     assert(aems_equal_upto epmax itsl);
@@ -41,7 +41,7 @@ let lemma_verifier_correct
     if is_eac itsl_ep then (
       (* is_eac itsl_ep ==> this sequence is sequentially consistent *)
       lemma_eac_implies_appfn_calls_seq_consistent itsl_ep;
-      assert(seq_consistent (G.appfn_calls (to_glog itsl_ep)));
+      assert(seq_consistent (G.app_fcrs (to_glog itsl_ep)));
 
       hash_collision_contra app
     )
