high2/Zeta.SeqConsistent.fst
@@ -3,6 +3,8 @@ module Zeta.SeqConsistent
 open FStar.Seq
 open Zeta.Interleave
 open Zeta.App
+open Zeta.AppSimulate
+open Zeta.AppSimulate.Helper
 open Zeta.Key
 open Zeta.GenKey
 open Zeta.Record
@@ -23,68 +25,130 @@ module SA = Zeta.SeqAux
 module EAC=Zeta.EAC
 module MSD = Zeta.MultiSetHashDomain
 
-open Zeta.AppSimulate
-open Zeta.AppSimulate.Helper
 
+(* TODO: Move to Generic.Interleave *)
 let lemma_appfn_calls_interleave (#app #n:_) (il: verifiable_log app n)
-  : Lemma (ensures (let cril = appfn_calls_il il in
+  : Lemma (ensures (let fcrs_il = app_fcrs_il il in
                     let gl = to_glog il in
-                    s_seq cril = G.appfn_calls gl))
-          [SMTPat (appfn_calls_il il)]
+                    s_seq fcrs_il = G.app_fcrs gl))
+          [SMTPat (app_fcrs_il il)]
   = admit()
 
-let appfn_calls_empty (#app #n:_) (il: verifiable_log app n)
-  : Lemma (ensures (length il = 0 ==> S.length (appfn_calls il) = 0))
+(* TODO: Move to Generic.Interleave *)
+let app_fcrs_empty (#app #n:_) (il: verifiable_log app n)
+  : Lemma (ensures (length il = 0 ==> S.length (app_fcrs il) = 0))
   = admit()
 
+(* TODO: Move to Generic.Interleave *)
 let appfn_calls_snoc (#app #n:_) (il: verifiable_log app n {length il > 0})
   : Lemma (ensures (let i = length il - 1 in
                     let e = index il i in
                     let il' = prefix il i in
-                    let cr = appfn_calls il in
-                    let cr' = appfn_calls il' in
+                    let cr = app_fcrs il in
+                    let cr' = app_fcrs il' in
                     match e with
-                    | RunApp _ _ _ -> cr == SA.append1 cr' (to_appfn_call_res il i)
+                    | RunApp _ _ _ -> cr == SA.append1 cr' (to_app_fcr il i)
                     | _ -> cr == cr'))
   = admit()
 
+let eac_app_state (#app #n:_) (il: eac_log app n) (ak: app_key app.adm)
+  = let gk = AppK ak in
+    AppV?.v (eac_value gk il)
+
+let to_fc (#app #n:_) (il: eac_log app n) (i: seq_index il {RunApp? (index il i)})
+  : appfn_call app
+  = let App (RunApp fid_c arg_c _) inp_c = mk_vlog_entry_ext il i in
+    { fid_c; arg_c ; inp_c }
+
+let eac_implies_appfn_success (#app #n:_) (il: eac_log app n) (i: seq_index il {RunApp? (index il i)})
+  : Lemma (ensures (correct (to_fc il i)))
+          [SMTPat (to_fc il i)]
+  = let open Zeta.BinTree in
+    eac_state_transition Root il i
+
+let eac_app_prop (#app #n:_) (il: eac_log app n)
+  = let fcrs = app_fcrs il in
+    let fcs = app_fcs fcrs in
+    (* the results are valid meaning the output corresponds to the input records *)
+    valid_call_result fcrs /\
+    (* the app state as recorded by eac values is the same as the simulation state *)
+    post_state fcs == eac_app_state il
+
+(* TODO: Move to AppSimulate.Helper *)
 let empty_call_result_valid (#app) (rs: seq (appfn_call_res app))
   : Lemma (ensures (S.length rs = 0 ==> valid_call_result rs))
   = admit()
 
-let eac_implies_appfn_valid_empty (#app #n:_) (il: eac_log app n)
-  : Lemma (ensures (length il = 0 ==> valid_call_result (appfn_calls il)))
+let eac_app_prop_empty (#app #n:_) (il: eac_log app n)
+  : Lemma (ensures (length il = 0 ==> eac_app_prop il))
   = if length il = 0 then (
-      appfn_calls_empty il;
-      empty_call_result_valid (appfn_calls il)
+      app_fcrs_empty il;
+      empty_call_result_valid (app_fcrs il);
+
+      let aux (ak:key app)
+        : Lemma (ensures (True))
+        = admit()
+      in
+      admit()
     )
 
-let eac_implies_appfn_valid_snoc (#app #n:_) (il: eac_log app n {length il > 0})
-  : Lemma (requires (let i = length il - 1 in
-                     let il' = prefix il i in
-                     valid_call_result (appfn_calls il')))
-          (ensures (valid_call_result (appfn_calls il)))
+let eac_app_state_key_snoc (#app #n:_) (il: eac_log app n {length il > 0}) (ak: app_key app.adm)
+  : Lemma (ensures (let i = length il - 1 in
+                    let e = index il i in
+                    let il' = prefix il i in
+                    match e with
+                    | RunApp f p ss ->
+                      let fc = to_fc il i in
+                      if fc `refs_comp` ak then
+                        eac_app_state il ak = write fc ak
+                      else
+                        eac_app_state il ak = eac_app_state il' ak
+                    | _ -> eac_app_state il ak = eac_app_state il' ak))
+  = admit()
+
+let eac_app_state_nonapp_snoc (#app #n:_) (il: eac_log app n {length il > 0})
+  : Lemma (ensures (let i = length il - 1 in
+                    let il' = prefix il i in
+                    not (RunApp? (index il i)) ==>
+                    eac_app_state il == eac_app_state il'))
   = let i = length il - 1 in
     let il' = prefix il i in
-    let cr = appfn_calls il in
-    let cr' = appfn_calls il' in
+    let e = index il i in
+    if not (RunApp? e) then (
+      let aux (ak:_)
+        : Lemma (ensures (eac_app_state il ak = eac_app_state il' ak))
+        = eac_app_state_key_snoc il ak
+      in
+      FStar.Classical.forall_intro aux;
+      assert(app_state_feq (eac_app_state il) (eac_app_state il'))
+    )
+
+let eac_implies_app_prop_snoc (#app #n:_) (il: eac_log app n {length il > 0})
+  : Lemma (requires (let i = length il - 1 in
+                     let il' = prefix il i in
+                     eac_app_prop il'))
+          (ensures eac_app_prop il)
+  = let i = length il - 1 in
+    let il' = prefix il i in
+    let fcrs = app_fcrs il in
+    let fcrs' = app_fcrs il' in
     let e = index il i in
     appfn_calls_snoc il;
+    eac_app_state_nonapp_snoc il;
 
     match e with
     | RunApp f p ss -> admit()
     | _ -> ()
 
-let rec eac_implies_appfn_valid (#app #n:_) (il: eac_log app n)
-  : Lemma (ensures (let cr = appfn_calls il in
-                    valid_call_result cr))
+let rec eac_implies_app_prop (#app #n:_) (il: eac_log app n)
+  : Lemma (ensures (eac_app_prop il))
           (decreases (length il))
-  = eac_implies_appfn_valid_empty il;
+  = eac_app_prop_empty il;
     if length il > 0 then (
       let i = length il - 1 in
       let il' = prefix il i in
-      eac_implies_appfn_valid il';
-      eac_implies_appfn_valid_snoc il
+      eac_implies_app_prop il';
+      eac_implies_app_prop_snoc il
     )
 
 let interleaving_implies_interleave (#a #n:_) (il: interleaving a n)
@@ -95,12 +159,12 @@ let interleaving_implies_interleave (#a #n:_) (il: interleaving a n)
 
 let lemma_eac_implies_appfn_calls_seq_consistent (#app #n:_) (il: eac_log app n)
   : Lemma (ensures (let gl = to_glog il in
-                    Zeta.AppSimulate.seq_consistent (G.appfn_calls gl)))
-  = let cr_il = appfn_calls_il il in
-    let crs = i_seq cr_il in
-    let crss = s_seq cr_il in
-    interleaving_implies_interleave cr_il;
-    assert(interleave crs crss);
-    eac_implies_appfn_valid il;
-    assert(valid_call_result crs);
-    FStar.Classical.exists_intro (fun is -> interleave #(appfn_call_res app) is crss) crs
+                    Zeta.AppSimulate.seq_consistent (G.app_fcrs gl)))
+  = let fcrs_il = app_fcrs_il il in
+    let fcrs = i_seq fcrs_il in
+    let fcrss = s_seq fcrs_il in
+    interleaving_implies_interleave fcrs_il;
+    assert(interleave fcrs fcrss);
+    eac_implies_app_prop il;
+    assert(valid_call_result fcrs);
+    FStar.Classical.exists_intro (fun is -> interleave #(appfn_call_res app) is fcrss) fcrs
