high2/Zeta.High.Interleave.fsti
@@ -345,4 +345,4 @@ val eac_fail_key (#app #n:_) (il: neac_log app n)
 
 val lemma_eac_implies_appfn_calls_seq_consistent (#app #n:_) (il: eac_log app n)
   : Lemma (ensures (let gl = to_glog il in
-                    Zeta.AppSimulate.seq_consistent (G.appfn_calls gl)))
+                    Zeta.AppSimulate.seq_consistent (G.app_fcrs gl)))
