utils/Zeta.SeqIdx.fsti
@@ -15,12 +15,13 @@ val exists_elems_with_prop_intro (#a:_) (p: a -> bool) (s: seq a) (i: seq_index 
 val last_idx (#a:_) (p: a -> bool) (s: seq a {exists_elems_with_prop p s})
   : i:seq_index s{p (index s i)}
 
-val last_idx_snoc (#a:_) (p: a -> bool) (s: seq a {exists_elems_with_prop p s /\ length s > 0})
+val last_idx_snoc (#a:_) (p: a -> bool) (s: seq a {length s > 0})
   : Lemma (ensures (let i = length s - 1 in
                     let s' = prefix s i in
                     p (index s i) /\ last_idx p s = i \/
-                    ~ (p (index s i)) /\ exists_elems_with_prop p s' /\
-                    last_idx p s = last_idx p s'))
+                    ~ (p (index s i))  /\
+                    (exists_elems_with_prop p s <==> exists_elems_with_prop p s') /\
+                    (exists_elems_with_prop p s' ==> last_idx p s = last_idx p s')))
 
 val last_idx_correct (#a:_) (p: a -> bool)
   (s: seq a{exists_elems_with_prop p s})
